Test/civl/samples/2pc.bpl
@@ -41,38 +41,38 @@ axiom 0 < n;
 axiom (forall xid1: TransactionId, xid2: TransactionId :: Conflict[xid1][xid2] == Conflict[xid2][xid1]);
 axiom (forall xid0: TransactionId :: Conflict[xid0][xid0] == true);
 
-var {:layer 0,1} locked_transactions: [ReplicaId](Set TransactionId);
-var {:layer 0,1} committed_transactions: Set TransactionId;
+var {:layer 0,1} locked_transactions: [ReplicaId]([TransactionId]bool);
+var {:layer 0,1} committed_transactions: [TransactionId]bool;
 
-function noConflicts(xids: (Set TransactionId), xid: TransactionId) : bool
+function noConflicts(xids: [TransactionId]bool, xid: TransactionId) : bool
 {
     !(exists x: TransactionId :: Set_Contains(xids, x) && Conflict[x][xid])
 }
 
-function {:inline} VoteRequests(xid: TransactionId, i: int, j: int) : Set (One VoteRequest)
+function {:inline} VoteRequests(xid: TransactionId, i: int, j: int) : [One VoteRequest]bool
 {
-    Set((lambda vr: One VoteRequest :: vr->val->xid == xid &&  i <= vr->val->rid && vr->val->rid <= j))
+    (lambda vr: One VoteRequest :: vr->val->xid == xid &&  i <= vr->val->rid && vr->val->rid <= j)
 }
 
-function allVoteRequests(xid: TransactionId) : Set (One VoteRequest)
+function allVoteRequests(xid: TransactionId) : [One VoteRequest]bool
 {
     VoteRequests(xid, 1, n)
 }
 
-function remainingVoteRequests(xid: TransactionId, i: int) : Set (One VoteRequest)
+function remainingVoteRequests(xid: TransactionId, i: int) : [One VoteRequest]bool
 {
     VoteRequests(xid, i, n)
 }
 
-yield procedure {:layer 1} TPC({:linear} xid: One TransactionId, {:linear_in} vrs: (Set (One VoteRequest)))
-requires {:layer 1} vrs == allVoteRequests(xid->val);
+yield procedure {:layer 1} TPC({:linear} xid: One TransactionId, {:linear_in} vrs: (UnitMap (One VoteRequest)))
+requires {:layer 1} vrs->dom == allVoteRequests(xid->val);
 requires call LockedNoConflicts();
 requires call CommittedSubsetLocked();
 requires call XidNotInCommitted(xid);
 {
     var d: Decision;
     var votes: [ReplicaId]Vote;
-    var vrs': Set (One VoteRequest);
+    var vrs': UnitMap (One VoteRequest);
     var i: int;
 
     d := COMMIT();
@@ -101,13 +101,13 @@ requires call XidNotInCommitted(xid);
     }
 }
 
-yield right procedure {:layer 1} vote_all(xid: TransactionId, {:linear_in} vrs: Set (One VoteRequest), i: int) returns (votes: [ReplicaId]Vote, {:linear} vrs': Set (One VoteRequest))
-requires {:layer 1} vrs == VoteRequests(xid, 1, i);
+yield right procedure {:layer 1} vote_all(xid: TransactionId, {:linear_in} vrs: UnitMap (One VoteRequest), i: int) returns (votes: [ReplicaId]Vote, {:linear} vrs': UnitMap (One VoteRequest))
+requires {:layer 1} vrs->dom == VoteRequests(xid, 1, i);
 ensures {:layer 1} (forall j:int :: 1 <= j && j < i+1 && votes[j] == YES() ==> Set_Contains(locked_transactions[j], xid));
-ensures {:layer 1} vrs' == VoteRequests(xid, 1, i);
+ensures {:layer 1} vrs'->dom == VoteRequests(xid, 1, i);
 preserves {:layer 1} LockedNoConflicts(locked_transactions);
 preserves {:layer 1} CommittedSubsetLocked(locked_transactions, committed_transactions);
-ensures {:layer 1} (forall j:int :: 1 <= j && j < n+1 ==> IsSubset(old(locked_transactions)[j]->val, locked_transactions[j]->val));
+ensures {:layer 1} (forall j:int :: 1 <= j && j < n+1 ==> Set_IsSubset(old(locked_transactions)[j], locked_transactions[j]));
 ensures {:layer 1} (forall j:int :: 1 <= j && j < i+1 ==> votes[j] != NONE());
 modifies locked_transactions;
 {
@@ -125,8 +125,8 @@ modifies locked_transactions;
     }
 }
 
-yield left procedure {:layer 1} finalize_all(d: Decision, {:linear} xid: One TransactionId, {:linear_in} vrs: Set (One VoteRequest))
-requires {:layer 1} vrs == allVoteRequests(xid->val);
+yield left procedure {:layer 1} finalize_all(d: Decision, {:linear} xid: One TransactionId, {:linear_in} vrs: UnitMap (One VoteRequest))
+requires {:layer 1} vrs->dom == allVoteRequests(xid->val);
 requires {:layer 1}  (forall j:int :: {:add_to_pool "J", j} d == COMMIT() &&  1 <= j && j < n+1 ==> Set_Contains(locked_transactions[j], xid->val));
 ensures {:layer 1}  (forall j:int :: d == COMMIT() && 1 <=j && j < n+1 ==> Set_Contains(locked_transactions[j], xid->val));
 preserves {:layer 1} LockedNoConflicts(locked_transactions);
@@ -137,7 +137,7 @@ modifies locked_transactions;
 {
     var i: int;
     var vr: One VoteRequest;
-    var vrs': Set (One VoteRequest);
+    var vrs': UnitMap (One VoteRequest);
 
     vrs' := vrs;
     i := 1;
@@ -145,7 +145,7 @@ modifies locked_transactions;
     while (i <= n)
     invariant {:layer 1} (forall j:int :: d == COMMIT() && 1 <= j && j < i ==> Set_Contains(locked_transactions[j], xid->val));
     invariant {:layer 1} (forall j:int :: d == COMMIT() && (i <= j) && (j < n+1)  ==> Set_Contains(locked_transactions[j], xid->val));
-    invariant {:layer 1} vrs' == remainingVoteRequests(xid->val, i);
+    invariant {:layer 1} vrs'->dom == remainingVoteRequests(xid->val, i);
     invariant {:layer 1} (forall  j:int,  xid1: TransactionId, xid2: TransactionId :: (1 <= j && j < n+1 && xid1 != xid2 && Set_Contains(locked_transactions[j], xid1) && Set_Contains(locked_transactions[j], xid2)) ==> !Conflict[xid1][xid2]);
     invariant {:layer 1} (forall j:int, xid0: TransactionId ::  1 <= j && j < n+1 && Set_Contains(committed_transactions, xid0) ==> Set_Contains(locked_transactions[j], xid0));
     invariant {:layer 1} !Set_Contains(committed_transactions, xid->val);
@@ -192,7 +192,7 @@ refines atomic action {:layer 1, 1} _ {
     committed_transactions := Set_Add(committed_transactions, xid->val);
 }
 
-function {:inline} LockedNoConflicts(locked_transactions: [ReplicaId](Set TransactionId)) : bool
+function {:inline} LockedNoConflicts(locked_transactions: [ReplicaId][TransactionId]bool) : bool
 {
     (forall  {:pool "J"} j: int, xid1: TransactionId, xid2: TransactionId :: {:add_to_pool "J", j}
         1 <= j && j < n+1 && xid1 != xid2 && Set_Contains(locked_transactions[j], xid1) && Set_Contains(locked_transactions[j], xid2)
@@ -201,7 +201,7 @@ function {:inline} LockedNoConflicts(locked_transactions: [ReplicaId](Set Transa
 yield invariant {:layer 1} LockedNoConflicts();
 preserves {:layer 1} LockedNoConflicts(locked_transactions);
 
-function {:inline} CommittedSubsetLocked(locked_transactions: [ReplicaId](Set TransactionId), committed_transactions: Set TransactionId) : bool
+function {:inline} CommittedSubsetLocked(locked_transactions: [ReplicaId][TransactionId]bool, committed_transactions: [TransactionId]bool) : bool
 {
     (forall {:pool "J"} j: int, xid0: TransactionId :: {:add_to_pool "J", j}
         1 <= j && j < n+1 && Set_Contains(committed_transactions, xid0)
