Test/civl/samples/PingPong.bpl
@@ -23,7 +23,7 @@ var {:layer 0,1} channels: [ChannelId]ChannelPair;
 // Right permission is used to receive from the right channel and send to the left channel.
 datatype ChannelHandle { Left(cid: ChannelId), Right(cid: ChannelId) }
 
-function {:inline} BothHandles(cid: ChannelId): Set (One ChannelHandle)
+function {:inline} BothHandles(cid: ChannelId): [One ChannelHandle]bool
 { Set_Add(Set_Singleton(One(Left(cid))), One(Right(cid))) }
 
 function {:inline} Empty() : [int]int { MapConst(0) }
@@ -32,8 +32,8 @@ function {:inline} Singleton(x: int): [int]int { Empty()[x := 1] }
 
 ////////////////////////////////////////////////////////////////////////////////
 
-yield invariant {:layer 1} YieldMain(cid: ChannelId, {:linear} handles: Set (One ChannelHandle));
-preserves handles == BothHandles(cid);
+yield invariant {:layer 1} YieldMain(cid: ChannelId, {:linear} handles: UnitMap (One ChannelHandle));
+preserves handles->dom == BothHandles(cid);
 preserves channels[cid] == ChannelPair(Empty(), Empty());
 
 yield invariant {:layer 1} YieldPing(x: int, {:linear} p: One ChannelHandle);
@@ -53,10 +53,10 @@ preserves (var left_channel, right_channel := channels[p->val->cid]->left, chann
 ////////////////////////////////////////////////////////////////////////////////
 
 yield procedure {:layer 1}
-main (cid: ChannelId, {:linear_in} handles: Set (One ChannelHandle))
+main (cid: ChannelId, {:linear_in} handles: UnitMap (One ChannelHandle))
 requires call YieldMain(cid, handles);
 {
-  var handles': Set (One ChannelHandle);
+  var handles': UnitMap (One ChannelHandle);
   var left: One ChannelHandle;
   var right: One ChannelHandle;
 
